new theorems, new GenCodable typeclass programming in order to automatically generate Codable instances, separating the API for Codable from the API for WType, added terms that eliminate the use of lambda functions when creating Code or Univ because it messes up typeclass synthesis for GenCodable, other misc changes

Mystdlib/Univ/Basic.lean
@@ -27,6 +27,9 @@ theorem mem_iff_mem_arities
 
 def get (k : String) (univ : Univ) (h : k ∈ univ) : (n : Nat) × (Vector Type n -> Type) :=
   univ.inner.get k (by simp_all [Membership.mem])
+
+def get? (k : String) (univ : Univ) :=
+  univ.inner.get? k
     
 def getArity (k : String) (univ : Univ) (h : k ∈ univ) : Nat :=
   (univ.inner.get k (by simp_all [Membership.mem])).1
@@ -37,8 +40,42 @@ def getInterpretation (k : String) (univ : Univ) (h : k ∈ univ) : Vector Type 
 
 abbrev Code := WType.Free String
 
+namespace Code
+
+def repr (code : Code) : String :=
+  code.elim _ fun ⟨head, tail⟩ =>
+    if head.2 = 0
+    then head.1
+    else "(" ++ head.1 ++ " " ++ String.intercalate " " (List.ofFn tail) ++ ")"
+
+instance : Repr Code where
+  reprPrec := fun x _ => x.repr
+
+def head (code : Code) : String × Nat := 
+  WType.head code
+
+def arity (code : Code) : Nat := 
+  code.head.2
+
+def typ (code : Code) : String :=
+  code.head.1
+
+def tail (code : Code) : Fin code.arity -> Code :=
+  fun fin => (WType.tail code) fin
+
+abbrev mk (typ : String) (arity : Nat) (subterms : List Code) (h : subterms.length = arity := by simp) : Code :=
+  WType.mk (typ, arity) (h ▸ subterms.get)
+
+instance : EmptyCollection (Vector Code 0) where
+  emptyCollection := ⟨#[], by simp⟩
+
+abbrev mk' (typ : String) : Code := 
+  WType.mk (typ, 0) (∅ : Vector Code 0).get
+
+end Code
+
 inductive SatisfiedBy (univ : Univ) : Code -> Prop 
-| intro {codeNode : String} : (h : codeNode ∈ univ) -> (cont : Fin (univ.getArity codeNode h) -> Code) -> (∀i, univ.SatisfiedBy (cont i)) -> univ.SatisfiedBy (.mk (codeNode, univ.getArity codeNode h) cont)
+| intro {codeNode : String} : (h : codeNode ∈ univ) -> (cont : Fin (univ.getArity codeNode h) -> Code) -> (∀i, univ.SatisfiedBy (cont i)) -> univ.SatisfiedBy (WType.mk (codeNode, univ.getArity codeNode h) cont)
 
 
 theorem SatisfiedBy_congr_aux
@@ -80,7 +117,7 @@ theorem not_SatisfiedBy_of_not_mem
   : ¬ code.head.fst ∈ univ -> ¬ univ.SatisfiedBy code := by
     intro h wf
     cases wf
-    simp [WType.head] at h
+    simp [Code.head, WType.head] at h
     grind
 
 theorem not_SatisfiedBy_of_get_neq_arity
@@ -100,7 +137,7 @@ theorem not_SatisfiedBy_of_child_not_wf
   : ¬ univ.SatisfiedBy (code.tail i) -> ¬ univ.SatisfiedBy code := by
     intro h wf
     cases wf
-    simp [WType.tail] at h
+    simp [Code.tail, WType.tail] at h
     grind
 
 theorem not_SatisfiedBy_of_child_not_mem
@@ -116,7 +153,7 @@ theorem not_SatisfiedBy_of_child_not_mem
 
 def SatisfiedBy_decidable {univ : Univ} : Decidable (univ.SatisfiedBy code) :=
   match hmatch : code with
-  | .mk (fst, snd) tail =>
+  | WType.mk (fst, snd) tail =>
     if h : ∀i, (SatisfiedBy_decidable (code := tail i) (univ := univ)).decide = true
     then if h' : fst ∈ univ
       then if h'' : univ.getArity fst h' = snd
@@ -125,7 +162,7 @@ def SatisfiedBy_decidable {univ : Univ} : Decidable (univ.SatisfiedBy code) :=
           grind [SatisfiedBy.intro]
         else .isFalse <| by
           apply not_SatisfiedBy_of_get_neq_arity
-          <;> grind [WType.head]
+          <;> grind [Code.head, WType.head]
       else .isFalse <| by
         apply not_SatisfiedBy_of_not_mem h'
     else .isFalse <| by
@@ -168,10 +205,31 @@ def decode (univ : Univ) (code : Univ.Code) (h : univ.SatisfiedBy code) : Type :
 where finally
   all_goals (cases h; subst aux; simp [Univ.getArity, Univ.get])
 
+def decode? (univ : Univ) (code : Univ.Code) : Option Type :=
+  if h : univ.SatisfiedBy code
+  then decode univ code h
+  else .none
+
 def Domain (univ : Univ) := { code // univ.SatisfiedBy code }
 
 def Domain.decode {univ : Univ} (code : univ.Domain) : Type := 
   univ.decode code.val code.property
+
+structure CodedTerm (univ : Univ) where
+  code : Code
+  satisfies : univ.SatisfiedBy code
+  term : univ.decode code satisfies
+
+def CodedTerm.type (ct : CodedTerm univ) : Type :=
+  univ.decode ct.code ct.satisfies
+
+structure Domain.Term (domcode : Domain univ) where
+  term : domcode.decode
+
+def Domain.Term.toCodedTerm {domcode : Univ.Domain univ} (t : domcode.Term) : univ.CodedTerm where
+  code := domcode.val
+  satisfies := domcode.property
+  term := t.term
 
 instance : Union Univ where
   union := fun univ univ' => ⟨univ.inner ∪ univ'.inner⟩
@@ -213,6 +271,30 @@ theorem getArity_union_of_mem_right
     congr 1
     apply DMap.getValueCast_union_of_mem_right
 
+
+theorem getArity_union_of_mem_left_and_not_mem_right
+  {x y : Univ}
+  (mem : k ∈ x)
+  (notmem : k ∉ y)
+  : (x ∪ y).getArity k (by grind [mem_union_of_left]) = x.getArity k mem := by
+    simp [getArity]
+    congr 1
+    apply Map.getValueCast_union_of_mem_left_and_not_mem_right
+      (by simp [mem_iff_mem_arities, arities, <- Map.mem_map] at mem; grind [Map.mem_union_of_left])
+      (by simp_all [Membership.mem])
+
+def Disjoint (x y : Univ) : Prop :=
+  ∀k, k ∈ x -> k ∉ y
+  deriving Decidable
+
+theorem getArity_Disjoint_union_of_mem_left
+  {x y : Univ}
+  (hdisj : x.Disjoint y)
+  (mem : k ∈ x)
+  : (x ∪ y).getArity k (by grind [mem_union_of_left]) = x.getArity k mem := by
+    apply getArity_union_of_mem_left_and_not_mem_right
+    grind [Disjoint]
+
 theorem satisfies_union_of_satisfies_right
   {x y : Univ}
   (h : y.SatisfiedBy code)
@@ -238,65 +320,105 @@ decreasing_by
     ⟨n, by grind⟩
   grind
 
+theorem satisfies_Disjoint_union_of_satisfies_left
+  {x y : Univ}
+  (hdisj : x.Disjoint y)
+  (satisfies : x.SatisfiedBy code)
+  : (x ∪ y).SatisfiedBy code := by
+    obtain ⟨ismem, tail, ih⟩ := satisfies
+    rename_i codeNode
+    suffices getArity codeNode x ismem = getArity codeNode (x ∪ y) (by grind [mem_union_of_left]) by
+      rw [SatisfiedBy_congr_aux this]
+      constructor
+      rintro ⟨n, lt⟩
+      apply satisfies_Disjoint_union_of_satisfies_left
+      <;> simp_all
+    grind [getArity_Disjoint_union_of_mem_left]
+
 theorem union_decode_eq_right_decode
   {x y : Univ}
   {code : Code}
   {h : y.SatisfiedBy code}
   : (x ∪ y).decode code (satisfies_union_of_satisfies_right h) = y.decode code h := by
     induction code with | mk head tail ih => ?_
-    simp [decode]
+    simp only [decode]
     conv =>
       left
       right
       right
       intro i
       rw [ih (h := by cases h; grind)]
-    simp [get, Map.get]
+    simp only [get, Map.get]
     rw! (castMode := .all) [union_def]
-    simp
     rw! (castMode := .all) [Map.getValueCast_union_of_mem_right]
     · simp
     · have := head_mem_of_SatisfiedBy h
       simp_all [Membership.mem]
 
-class Codable (α : Type) (univ : Univ) where
-  code : Code
-  satisfies : univ.SatisfiedBy code
-  wf : univ.decode code satisfies = α := by simp
+theorem Disjoint_union_decode_eq_left_decode
+  {x y : Univ}
+  {code : Code}
+  {h : x.SatisfiedBy code}
+  (hdisj : x.Disjoint y)
+  : (x ∪ y).decode code (satisfies_Disjoint_union_of_satisfies_left hdisj h) = x.decode code h := by
+    induction code with | mk head tail ih => ?_
+    simp only [decode]
+    conv =>
+      left
+      right
+      right
+      intro i
+      rw [ih (h := by cases h; grind)]
+    simp only [get, Map.get]
+    rw! (castMode := .all) [union_def]
+    have := Map.getValueCast_union_of_mem_left_and_not_mem_right 
+      (by apply head_mem_of_SatisfiedBy h)
+      (by simp [Disjoint, mem_iff_mem_arities, arities, <- Map.mem_map] at hdisj; apply hdisj; apply head_mem_of_SatisfiedBy h)
+    rw! (castMode := .all) [this]
+    simp
 
-instance [inst : Codable α y] : Codable α (x ∪ y) where
-  code := inst.code
-  satisfies := satisfies_union_of_satisfies_right inst.satisfies
-  wf := by 
-    have := inst.wf
-    rw! (castMode := .all) (occs := [4]) [<- inst.wf]
-    apply union_decode_eq_right_decode
+class DisjointUnivUnion (x y : Univ) where
+  disjoint : x.Disjoint y
 
+instance {x y : Univ} : Coe y.CodedTerm (x ∪ y).CodedTerm where
+  coe := fun ⟨code, satisfies, term⟩ => ⟨code, Univ.satisfies_union_of_satisfies_right satisfies, cast (by symm; apply Univ.union_decode_eq_right_decode) term⟩
 
-def BasicUniv : Univ where
-  inner := .ofList [
-      ("nat", ⟨0, fun _ => Nat⟩),
-      ("bool", ⟨0, fun _ => Bool⟩),
-      ("unit", ⟨0, fun _ => Unit⟩),
-      ("empty", ⟨0, fun _ => Empty⟩),
-      ("string", ⟨0, fun _ => String⟩),
-      ("format", ⟨0, fun _ => Lean.Format⟩),
-      ("name", ⟨0, fun _ => Lean.Name⟩),
-      ("array", ⟨1, fun v => Array v[0]⟩),
-      ("list", ⟨1, fun v => List v[0]⟩),
-      ("prod", ⟨2, fun v => Prod v[0] v[1]⟩),
-      ("option", ⟨1, fun v => Option v[0]⟩)
-    ]
+instance [DisjointUnivUnion x y] : Coe x.CodedTerm (x ∪ y).CodedTerm where
+  coe := fun ⟨code, satisfies, term⟩ => ⟨code, Univ.satisfies_Disjoint_union_of_satisfies_left DisjointUnivUnion.disjoint satisfies, cast (by symm; apply Univ.Disjoint_union_decode_eq_left_decode; apply DisjointUnivUnion.disjoint) term⟩
 
+class Codable (α : Type) (univ : Univ) (code : outParam Code) where
+  satisfies : univ.SatisfiedBy code := by native_decide
+  wf : univ.decode code satisfies = α := by cbv
 
---- 
+instance [Codable α x code] [DisjointUnivUnion x y] : Codable α (x ∪ y) code where
+  satisfies := Univ.satisfies_Disjoint_union_of_satisfies_left DisjointUnivUnion.disjoint (Codable.satisfies α)
+  wf := by
+    rw! [<- Codable.wf (α := α) (univ := x) (code := code)]
+    apply Univ.Disjoint_union_decode_eq_left_decode
+    apply DisjointUnivUnion.disjoint
 
-/-
-def wfterm (term : Univ.Code × Type) (univ : Univ) (h : univ.SatisfiedBy term.1) : Prop :=
-  term.2 = univ.decode term.1 h
+instance [Codable α y code] : Codable α (x ∪ y) code where
+  satisfies := Univ.satisfies_union_of_satisfies_right (Codable.satisfies α)
+  wf := by
+    rw! [<- Codable.wf (α := α) (univ := y) (code := code)]
+    apply Univ.union_decode_eq_right_decode
 
-example : wfterm (.mk ("nat", 0) nofun, Nat) BasicUniv (by native_decide) := by
-  unfold wfterm
-  simp
-  cbv
--/
+def mkTerm [Codable α univ code] (a : α) : univ.CodedTerm :=
+  ⟨code, Codable.satisfies α, cast (by symm; apply Codable.wf) a⟩
+
+class TypeFnGen (arity : Nat) (typ : outParam (Type 1)) where
+  fn : (F : typ) -> Vector Type arity -> Type
+
+instance : TypeFnGen 0 Type where
+  fn := fun t _ => t
+
+instance
+  [inst : TypeFnGen n t]
+  : TypeFnGen (Nat.succ n) (Type -> t) where
+    fn := fun F v =>
+      have := inst.fn
+      this (F v.head) v.tail
+
+def mkUnivEntry (typ : String) (arity : Nat) [TypeFnGen arity t] (F : t) : String ×  (n : Nat) × (Vector Type n -> Type) :=
+  (typ, ⟨arity, TypeFnGen.fn F⟩)
+
