Mystdlib/Univ/GenCodable.lean
@@ -1,0 +1,83 @@
+import Mystdlib.Univ.Basic
+
+open Univ
+
+class GenCodable (t : Type 1) (T : t) (types : List Type) (univ : Univ) (code : outParam Code)  where
+  satisfies : univ.SatisfiedBy code
+  eq : (h : t = Type) -> univ.decode code satisfies = h ▸ T
+
+instance : GenCodable Type T [] ⟨.ofList [mkUnivEntry typ 0 T]⟩ (.mk typ 0 []) := sorry
+
+instance 
+  [GenCodable t T v ⟨.ofList as⟩ code]
+  : GenCodable t T v ⟨.ofList (a :: as)⟩ code := sorry
+
+instance 
+  [GenCodable t T v ⟨.ofList (a :: as)⟩ code]
+  : GenCodable t T v ⟨.ofList (a :: b :: as)⟩ code := sorry
+
+class GenCodableAggregator (types : List Type) (univ : Univ) (len : outParam Nat) (codes : outParam (List Code)) where
+  wf1 : types.length = codes.length
+  wf2 : codes.length = len
+
+instance 
+  [GenCodable Type T [] univ code]
+  : GenCodableAggregator [T] univ 1 [code] := sorry
+
+instance
+  [GenCodableAggregator types univ n codes]
+  [GenCodable Type T [] univ code]
+  : GenCodableAggregator (T :: types) univ (Nat.succ n) (code :: codes) := sorry
+
+class IsUnivMem (t : Type 1) (α : t) (univ : Univ) (typ : outParam String)
+
+instance [TypeFnGen arity t] : IsUnivMem t α ⟨.ofList [mkUnivEntry typ arity α]⟩ typ where
+
+instance 
+  [IsUnivMem t α ⟨.ofList es⟩ a] 
+  : IsUnivMem t α ⟨.ofList (e :: es)⟩ a := sorry
+
+instance 
+  [IsUnivMem t α ⟨.ofList (e :: es)⟩ a]
+  : IsUnivMem t α ⟨.ofList (e :: e' :: es)⟩ a  := sorry
+
+instance
+  [TypeFnGen arity t]
+  [inst : GenCodableAggregator types univ arity codes]
+  [IsUnivMem t F univ f]
+  : GenCodable t F types univ (.mk f arity codes inst.wf2) := sorry
+
+instance 
+  [GenCodable (Type -> t) F (type :: types) univ code]
+  : GenCodable t (F type) types univ code := sorry
+
+
+instance 
+  [GenCodable Type T [] univ code]
+  : Codable T univ code := sorry
+
+
+--these two are needed because anonymous functions mess up synthesis
+instance
+  [GenCodable (Type -> Type -> Type) (· -> ·) [α, β] univ code]
+  : GenCodable (Type -> Type) (α -> ·) [β] univ code := sorry
+
+instance
+  {α β : Type}
+  [GenCodable (Type -> Type) (α -> ·) [β] univ code]
+  : GenCodable Type (α -> β) [] univ code := sorry
+
+
+
+/-
+abbrev BasicUniv : Univ where
+  inner := .ofList [
+      (mkUnivEntry "nat" 0 Nat),
+      (mkUnivEntry "bool" 0 Bool),
+      (mkUnivEntry "list" 1 List),
+      (mkUnivEntry "prod" 2 Prod),
+      (mkUnivEntry "arrow" 2 (· -> ·)),
+      (mkUnivEntry "string" 0 String),
+      ]
+
+-/
