Mystdlib/Univ/Structure.lean
@@ -1,4 +1,4 @@
-import Mystdlib.Univ.Free.Basic
+import Mystdlib.Univ.Basic
 import Mystdlib.Decidable
 import Mystdlib.DMap.Map.Lemmas
 
@@ -27,16 +27,14 @@ def ofList (l : List (String × Univ.Code)) : Structure :=
 def fields (stct : Structure) : List String :=
   stct.toMap.keys
 
-
 def get (str : String) (stct : Structure) (h : str ∈ stct) : Univ.Code :=
   stct.toMap.get str h
 
 structure Term (univ : Univ) where
-  toMap : Map String ((code : univ.Domain) × code.decode)
+  toMap : Map String univ.CodedTerm
 
 instance : Membership String (Term univ) where
   mem := fun t str => str ∈ t.toMap
-
 
 theorem Term.mem_iff_mem_toMap
   {stct : Term univ}
@@ -49,21 +47,13 @@ instance {str : String} {t : Term univ} : Decidable (str ∈ t) := by
   infer_instance
 
 def Term.getFieldCode (str : String) (t : Term univ) (h : str ∈ t) : Univ.Code :=
-  (t.toMap.get str h).fst.val
+  (t.toMap.get str h).code
 
 def Term.getFieldTerm (str : String) (t : Term univ) (h : str ∈ t) :=
-  (t.toMap.get str h).snd
+  (t.toMap.get str h).term
 
 def SatisfiedBy (stct : Structure) (term : Term univ) : Prop :=
   ∀(k : String) (h : k ∈ stct), ∃(h' : k ∈ term), stct.get k h = term.getFieldCode k h'
-
-instance {term : Term univ} {stct : Structure} : Decidable (∀k, k ∈ stct -> k ∈ term) := by
-  simp [mem_iff_mem_toMap, Term.mem_iff_mem_toMap]
-  infer_instance
-
-instance {term : Term univ} {stct : Structure} : Decidable (∀k, k ∈ term -> k ∈ stct) := by
-  simp [mem_iff_mem_toMap, Term.mem_iff_mem_toMap]
-  infer_instance
 
 instance : Decidable (SatisfiedBy stct term) := by
   unfold SatisfiedBy
